src/opt/Simulation.v
@@ -38,7 +38,7 @@ Section SimulationLocal.
   Qed.
   Next Obligation.
     ii. inv H. inv H0. econs.
-    - etransitivity; eauto.
+    - etrans; eauto.
     - apply MemInv.sem_bot_inv in PROMISE.
       apply MemInv.sem_bot_inv in PROMISE0.
       rewrite PROMISE, PROMISE0.
@@ -196,8 +196,8 @@ Lemma sim_thread_future
 Proof.
   pfold. ii.
   punfold SIM. exploit SIM; eauto.
-  - etransitivity; eauto.
-  - etransitivity; eauto.
+  - etrans; eauto.
+  - etrans; eauto.
 Qed.
 
 
@@ -211,8 +211,8 @@ Lemma sim_future
 Proof.
   pfold. ii.
   punfold SIM. exploit SIM; eauto.
-  - etransitivity; eauto.
-  - etransitivity; eauto.
+  - etrans; eauto.
+  - etrans; eauto.
 Qed.
 
 Lemma singleton_consistent
@@ -307,7 +307,7 @@ Proof.
   exploit IHSTEPS; eauto. i. des.
   destruct z. ss.
   eexists _, _, _. splits; try apply MEMORY1; eauto.
-  etransitivity; [eauto|]. econs 2; eauto.
+  etrans; [eauto|]. econs 2; eauto.
 Qed.
 
 Lemma sim_thread_consistent
@@ -332,7 +332,7 @@ Proof.
   punfold SIM0. exploit SIM0; eauto; try reflexivity. i. des.
   exploit PROMISE1; eauto. i. des.
   eexists (Thread.mk _ _ _ _). splits; [|eauto].
-  etransitivity; eauto.
+  etrans; eauto.
 Qed.
 
 
@@ -362,14 +362,14 @@ Proof.
         econs; ss; eauto.
         { eapply IdentMap.singleton_find. }
         { ii. eexists. splits; eauto. ss.
-          inv LOCAL. apply MemInv.sem_bot_inv in PROMISE0. etransitivity; eauto.
+          inv LOCAL. apply MemInv.sem_bot_inv in PROMISE0. etrans; eauto.
           apply THREAD.
         }
       * inv X. s. erewrite IdentMap.singleton_add. econs.
     + ii. ss. rewrite IdentMap.singleton_add in *.
       apply IdentMap.singleton_find_inv in FIND. des. subst.
       splits; Configuration.simplify. econs; eauto.
-      inv LOCAL. apply MemInv.sem_bot_inv in PROMISE0. etransitivity; eauto.
+      inv LOCAL. apply MemInv.sem_bot_inv in PROMISE0. etrans; eauto.
       apply THREAD.
   - i. inv STEP_TGT. ss.
     apply IdentMap.singleton_find_inv in TID. des.
@@ -381,7 +381,7 @@ Proof.
     eexists _, _, _, _. splits; eauto.
     + econs; s.
       * apply IdentMap.singleton_find.
-      * etransitivity; eauto.
+      * etrans; eauto.
       * eauto.
       * eapply sim_thread_consistent; eauto.
     + right. s. rewrite ? IdentMap.singleton_add.
